theories/lang/cpp/logic/new_delete.v
@@ -122,7 +122,7 @@ Module Type Expr__newdelete.
             new_fn new_args aty Q targs sz
             (nfty := normalize_type new_fn.2)
             (_ : arg_types nfty = Some (Tnum sz Unsigned :: targs, Ar_Definite)),
-            wp_args targs Ar_Definite new_args (fun vs free =>
+            wp_args (targs, Ar_Definite) new_args (fun vs free =>
                 Exists sz al, [| size_of aty = Some sz |] ** [| has_type sz Tsize_t |] ** [| align_of aty = Some al |] **
                 Reduce (alloc_size_t sz (fun p FR =>
                 |> fspec nfty (_global new_fn.1) (p :: vs) (fun res => FR $
@@ -182,7 +182,7 @@ Module Type Expr__newdelete.
               Exists array_sizeN, [| v = Vn array_sizeN |] **
                 (* The size must be greater than zero (see the quote from [expr.new#7] above). *)
                 [| 0 < array_sizeN |]%N **
-                wp_args targs Ar_Definite new_args (fun vs free' =>
+                wp_args (targs, Ar_Definite) new_args (fun vs free' =>
                   Exists sz al,
                     let array_ty := Tarray aty array_sizeN in
                     [| size_of array_ty = Some sz |] **
